Enable rw at hyps for nth_rewrite

src/tactic/rewrite_all/default.lean
@@ -7,20 +7,32 @@ Authors: Keeley Hoek, Scott Morrison
 import tactic.rewrite_all.congr
 
 /-!
-# `rewrite_all` tactic
+# Advanced rewriting tactics
+
+This file provides three interactive tactics
+that give the user more control over where to perform a rewrite.
+
+## Main definitions
+
+* `perform_nth_write n rules`: performs only the `n`th possible rewrite using the `rules`.
+* `nth_rewrite_lhs`: as above, but only rewrites on the left hand side of an equation or iff.
+* `nth_rewrite_rhs`: as above, but only rewrites on the right hand side of an equation or iff.
+
+## Implementation details
 
 There are two alternative backends, provided by `.congr` and `.kabstract`.
 The kabstract backend is not currently available through mathlib.
 
 The kabstract backend is faster, but if there are multiple identical occurences of the
-same rewritable subexpression, all are rewritten simultaneously, and this isn't always
-what we want.
+same rewritable subexpression, all are rewritten simultaneously,
+and this isn't always what we want.
 (In particular, `rewrite_search` is much less capable on the `category_theory` library.)
 -/
 
 open tactic
 open lean.parser
 open interactive
+open interactive.types
 
 namespace tactic
 
@@ -44,7 +56,7 @@ do e ← target,
    rewrites ← rewrite_all e r,
    rewrites.nth n
 
-meta def perform_nth_rewrite (r : expr × bool) (n : ℕ) : tactic unit :=
+meta def nth_rewrite (r : expr × bool) (n : ℕ) : tactic unit :=
 get_nth_rewrite r n >>= tracked_rewrite.replace_target
 
 meta def all_rewrites_using (a : name) (e : expr) :
@@ -66,6 +78,25 @@ private meta def get_nth_rewrite' (n : ℕ) (q : rw_rules_t) (e : expr) :
 do rewrites ← q.rules.mmap $ λ r, unpack_rule r >>= rewrite_all e,
    rewrites.join.nth n <|> fail format!"failed: not enough rewrites found"
 
+meta def nth_rw_hyp (n : parse small_nat) (q : parse rw_rules) (h : expr) : tactic unit :=
+do e ← infer_type h, get_nth_rewrite' n q e >>= tracked_rewrite.replace_hyp h
+
+-- TODO (also allow (%%lhs ↔ %%_))
+meta def nth_rw_hyp_lhs (n : parse small_nat) (q : parse rw_rules) (h : expr) : tactic unit :=
+do `(%%lhs = %%_) ← infer_type h, get_nth_rewrite' n q lhs >>= tracked_rewrite.replace_hyp_lhs h
+
+meta def nth_rw_hyp_rhs (n : parse small_nat) (q : parse rw_rules) (h : expr) : tactic unit :=
+do `(%%_ = %%rhs) ← infer_type h, get_nth_rewrite' n q rhs >>= tracked_rewrite.replace_hyp_rhs h
+
+meta def nth_rw_goal (n : parse small_nat) (q : parse rw_rules) : tactic unit :=
+do e ← target, get_nth_rewrite' n q e >>= tracked_rewrite.replace_target
+
+meta def nth_rw_goal_lhs (n : parse small_nat) (q : parse rw_rules) : tactic unit :=
+do `(%%lhs = %%_) ← target, get_nth_rewrite' n q lhs >>= tracked_rewrite.replace_target_lhs
+
+meta def nth_rw_goal_rhs (n : parse small_nat) (q : parse rw_rules) : tactic unit :=
+do `(%%_ = %%rhs) ← target, get_nth_rewrite' n q rhs >>= tracked_rewrite.replace_target_rhs
+
 /-- `perform_nth_write n rules` performs only the `n`th possible rewrite using the `rules`.
 
 The core `rewrite` has a `occs` configuration setting intended to achieve a similar
@@ -73,11 +104,13 @@ purpose, but this doesn't really work. (If a rule matches twice, but with differ
 values of arguments, the second match will not be identified.)
 
 See also: `nth_rewrite_lhs` and `nth_rewrite_rhs` -/
-meta def perform_nth_rewrite
-  (n : parse small_nat) (q : parse rw_rules) : tactic unit :=
-do e ← target,
-   get_nth_rewrite' n q e >>= tracked_rewrite.replace_target,
-   tactic.try tactic.reflexivity
+meta def nth_rewrite
+  (n : parse small_nat) (q : parse rw_rules) (l : parse location) : tactic unit :=
+match l with
+| loc.wildcard := l.try_apply (nth_rw_hyp n q) (nth_rw_goal n q)
+| _            := l.apply     (nth_rw_hyp n q) (nth_rw_goal n q)
+end >> tactic.try (tactic.reflexivity reducible)
+    >> (returnopt q.end_pos >>= save_info <|> skip)
 
 /-- `nth_write_lhs n rules` performs only the `n`th possible rewrite using the `rules`,
 but only working on the left hand side.
@@ -86,11 +119,13 @@ The core `rewrite` has a `occs` configuration setting intended to achieve a simi
 purpose, but this doesn't really work. (If a rule matches twice, but with different
 values of arguments, the second match will not be identified.)
 
-See also: `perform_nth_rewrite` and `nth_rewrite_rhs` -/
-meta def nth_rewrite_lhs (n : parse small_nat) (q : parse rw_rules) : tactic unit :=
-do `(%%lhs = %%_) ← target,
-   get_nth_rewrite' n q lhs >>= tracked_rewrite.replace_target_lhs,
-   tactic.try tactic.reflexivity
+See also: `nth_rewrite` and `nth_rewrite_rhs` -/
+meta def nth_rewrite_lhs (n : parse small_nat) (q : parse rw_rules) (l : parse location) : tactic unit :=
+match l with
+| loc.wildcard := l.try_apply (nth_rw_hyp_lhs n q) (nth_rw_goal_lhs n q)
+| _            := l.apply     (nth_rw_hyp_lhs n q) (nth_rw_goal_lhs n q)
+end >> tactic.try (tactic.reflexivity reducible)
+    >> (returnopt q.end_pos >>= save_info <|> skip)
 
 /-- `nth_write_rhs n rules` performs only the `n`th possible rewrite using the `rules`,
 but only working on the right hand side.
@@ -99,11 +134,13 @@ The core `rewrite` has a `occs` configuration setting intended to achieve a simi
 purpose, but this doesn't really work. (If a rule matches twice, but with different
 values of arguments, the second match will not be identified.)
 
-See also: `perform_nth_rewrite` and `nth_rewrite_lhs` -/
-meta def nth_rewrite_rhs (n : parse small_nat) (q : parse rw_rules) : tactic unit :=
-do `(%%_ = %%rhs) ← target,
-   get_nth_rewrite' n q rhs >>= tracked_rewrite.replace_target_rhs,
-   tactic.try tactic.reflexivity
+See also: `nth_rewrite` and `nth_rewrite_lhs` -/
+meta def nth_rewrite_rhs (n : parse small_nat) (q : parse rw_rules) (l : parse location) : tactic unit :=
+match l with
+| loc.wildcard := l.try_apply (nth_rw_hyp_rhs n q) (nth_rw_goal_rhs n q)
+| _            := l.apply     (nth_rw_hyp_rhs n q) (nth_rw_goal_rhs n q)
+end >> tactic.try (tactic.reflexivity reducible)
+    >> (returnopt q.end_pos >>= save_info <|> skip)
 
 end interactive
 end tactic
